theory/Static_Framework.thy
@@ -25,131 +25,6 @@ type_synonym step_label = "(node_label \<times> edge_label)"
 type_synonym static_path = "step_label list"
 
 
-inductive static_flow_set :: "abstract_value_env \<Rightarrow> flow_set \<Rightarrow> (var \<Rightarrow> node_label \<Rightarrow> bool) \<Rightarrow> exp \<Rightarrow> bool"  where
-  Result: "
-    static_flow_set V F is_recv_site (RESULT x)
-  " |
-  Let_Unit: "
-    \<lbrakk>
-      {(NLet x , ENext, nodeLabel e)} \<subseteq> F;
-      static_flow_set V F is_recv_site e
-    \<rbrakk> \<Longrightarrow>
-    static_flow_set V F is_recv_site (LET x = \<lparr>\<rparr> in e)
-  " |
-  Let_Chan: "
-    \<lbrakk>
-      {(NLet x, ENext, nodeLabel e)} \<subseteq> F;
-      static_flow_set V F is_recv_site e
-    \<rbrakk> \<Longrightarrow>
-    static_flow_set V F is_recv_site (LET x = CHAN \<lparr>\<rparr> in e)
-  " |
-  Let_Send_Evt: "
-    \<lbrakk>
-      {(NLet x, ENext, nodeLabel e)} \<subseteq> F;
-      static_flow_set V F is_recv_site e
-    \<rbrakk> \<Longrightarrow>
-    static_flow_set V F is_recv_site (LET x = SEND EVT x\<^sub>c x\<^sub>m in e)
-  " |
-  Let_Recv_Evt: "
-    \<lbrakk>
-      {(NLet x, ENext, nodeLabel e)} \<subseteq> F;
-      static_flow_set V F is_recv_site e
-    \<rbrakk> \<Longrightarrow>
-    static_flow_set V F is_recv_site (LET x = RECV EVT x\<^sub>c in e)
-  " |
-  Let_Pair: "
-    \<lbrakk>
-      {(NLet x, ENext, nodeLabel e)} \<subseteq> F;
-      static_flow_set V F is_recv_site e
-    \<rbrakk> \<Longrightarrow>
-    static_flow_set V F is_recv_site (LET x = \<lparr>x\<^sub>1, x\<^sub>2\<rparr> in e)
-  " |
-  Let_Left: "
-    \<lbrakk>
-      {(NLet x, ENext, nodeLabel e)} \<subseteq> F;
-      static_flow_set V F is_recv_site e
-    \<rbrakk> \<Longrightarrow>
-    static_flow_set V F is_recv_site (LET x = LEFT x\<^sub>p in e)
-  " |
-  Let_Right: "
-    \<lbrakk>
-      {(NLet x, ENext, nodeLabel e)} \<subseteq> F;
-      static_flow_set V F is_recv_site e
-    \<rbrakk> \<Longrightarrow>
-    static_flow_set V F is_recv_site (LET x = RIGHT x\<^sub>p in e)
-  " |
-  Let_Abs: "
-    \<lbrakk>
-      {(NLet x, ENext, nodeLabel e)} \<subseteq> F;
-      static_flow_set V F is_recv_site e\<^sub>b;
-      static_flow_set V F is_recv_site e
-    \<rbrakk> \<Longrightarrow>
-    static_flow_set V F is_recv_site (LET x = FN f x\<^sub>p . e\<^sub>b  in e)
-  " |
-  Let_Spawn: "
-    \<lbrakk>
-      {
-        (NLet x, ENext, nodeLabel e),
-        (NLet x, ESpawn, nodeLabel e\<^sub>c)
-      } \<subseteq> F;
-      static_flow_set V F is_recv_site e\<^sub>c;
-      static_flow_set V F is_recv_site e
-    \<rbrakk> \<Longrightarrow>
-    static_flow_set V F is_recv_site (LET x = SPAWN e\<^sub>c in e)
-  " |
-  Let_Sync: "
-    \<lbrakk>
-      {(NLet x, ENext, nodeLabel e)} \<subseteq> F;
-      (\<forall> xSC xM xC y.
-        {^Send_Evt xSC xM} \<subseteq> V x\<^sub>e \<longrightarrow>
-        {^Chan xC} \<subseteq> V xSC \<longrightarrow>
-        is_recv_site xC (NLet y) \<longrightarrow>
-        {(NLet x, ESend xSE, NLet y)} \<subseteq> F
-      );
-      static_flow_set V F is_recv_site e
-    \<rbrakk> \<Longrightarrow>
-    static_flow_set V F is_recv_site (LET x = SYNC xSE in e)
-  " |
-  Let_Fst: "
-    \<lbrakk>
-      {(NLet x, ENext, nodeLabel e)} \<subseteq> F;
-      static_flow_set V F is_recv_site e
-    \<rbrakk> \<Longrightarrow>
-    static_flow_set V F is_recv_site (LET x = FST x\<^sub>p in e)
-  " |
-  Let_Snd: "
-    \<lbrakk>
-      {(NLet x, ENext, nodeLabel e)} \<subseteq> F;
-      static_flow_set V F is_recv_site e
-    \<rbrakk> \<Longrightarrow>
-    static_flow_set V F is_recv_site (LET x = SND x\<^sub>p in e)
-  " |
-  Let_Case: "
-    \<lbrakk>
-      {
-        (NLet x, ECall x, nodeLabel e\<^sub>l),
-        (NLet x, ECall x, nodeLabel e\<^sub>r),
-        (NResult (\<lfloor>e\<^sub>l\<rfloor>), EReturn x, nodeLabel e),
-        (NResult (\<lfloor>e\<^sub>r\<rfloor>), EReturn x, nodeLabel e)
-      } \<subseteq> F;
-      static_flow_set V F is_recv_site e\<^sub>l;
-      static_flow_set V F is_recv_site e\<^sub>r;
-      static_flow_set V F is_recv_site e
-    \<rbrakk> \<Longrightarrow>
-    static_flow_set V F is_recv_site (LET x = CASE x\<^sub>s LEFT x\<^sub>l |> e\<^sub>l RIGHT x\<^sub>r |> e\<^sub>r in e)
-  " |
-  Let_App: "
-    \<lbrakk>
-      (\<forall> f' x\<^sub>p e\<^sub>b . ^Abs f' x\<^sub>p e\<^sub>b \<in> V f \<longrightarrow>
-        {
-          (NLet x, ECall x, nodeLabel e\<^sub>b),
-          (NResult (\<lfloor>e\<^sub>b\<rfloor>), EReturn x, nodeLabel e)
-        } \<subseteq> F);
-      static_flow_set V F is_recv_site e
-    \<rbrakk> \<Longrightarrow>
-    static_flow_set V F is_recv_site (LET x = APP f x\<^sub>a in e)
-  "
-
 inductive is_super_exp :: "exp \<Rightarrow> exp \<Rightarrow> bool"  where
   Refl : "
     is_super_exp e e
@@ -174,5 +49,175 @@ inductive is_super_exp :: "exp \<Rightarrow> exp \<Rightarrow> bool"  where
     is_super_exp e\<^sub>b e \<Longrightarrow>
     is_super_exp (LET x = FN f x\<^sub>p . e\<^sub>b in e\<^sub>n) e
   "
+
+
+lemma is_super_exp_trans: "
+  is_super_exp e\<^sub>z e\<^sub>y \<Longrightarrow> is_super_exp e\<^sub>y e\<^sub>x \<Longrightarrow> is_super_exp e\<^sub>z e\<^sub>x
+"
+proof -
+  assume "is_super_exp e\<^sub>y e\<^sub>x "
+  assume "is_super_exp e\<^sub>z e\<^sub>y" then
+  have "(\<forall> e\<^sub>x . is_super_exp e\<^sub>y e\<^sub>x \<longrightarrow> is_super_exp e\<^sub>z e\<^sub>x)"
+  proof (induction rule: is_super_exp.induct)
+    case (Refl e)
+    show "\<forall>e\<^sub>x. is_super_exp e e\<^sub>x \<longrightarrow> is_super_exp e e\<^sub>x" by simp
+  next
+    case (Let e\<^sub>n e x b)
+    assume "is_super_exp e\<^sub>n e" "\<forall>e\<^sub>x. is_super_exp e e\<^sub>x \<longrightarrow> is_super_exp e\<^sub>n e\<^sub>x"
+
+    have "\<forall>e\<^sub>x. is_super_exp e\<^sub>n e\<^sub>x \<longrightarrow> is_super_exp (LET x = b in e\<^sub>n) e\<^sub>x" by (simp add: is_super_exp.Let) 
+    with `\<forall>e\<^sub>x. is_super_exp e e\<^sub>x \<longrightarrow> is_super_exp e\<^sub>n e\<^sub>x`
+    show "\<forall>e\<^sub>x. is_super_exp e e\<^sub>x \<longrightarrow> is_super_exp (LET x = b in e\<^sub>n) e\<^sub>x" by blast
+  next
+    case (Let_Spawn_Child e\<^sub>c e x e\<^sub>n)
+    assume "is_super_exp e\<^sub>c e" "\<forall>e\<^sub>x. is_super_exp e e\<^sub>x \<longrightarrow> is_super_exp e\<^sub>c e\<^sub>x"
+
+    have "\<forall>e\<^sub>x. is_super_exp e\<^sub>c e\<^sub>x \<longrightarrow> is_super_exp (LET x = SPAWN e\<^sub>c in e\<^sub>n) e\<^sub>x" by (simp add: is_super_exp.Let_Spawn_Child)
+    with `\<forall>e\<^sub>x. is_super_exp e e\<^sub>x \<longrightarrow> is_super_exp e\<^sub>c e\<^sub>x`
+    show "\<forall>e\<^sub>x. is_super_exp e e\<^sub>x \<longrightarrow> is_super_exp (LET x = SPAWN e\<^sub>c in e\<^sub>n) e\<^sub>x"by blast
+  next
+    case (Let_Case_Left e\<^sub>l e x x\<^sub>s x\<^sub>l x\<^sub>r e\<^sub>r e\<^sub>n)
+    assume "is_super_exp e\<^sub>l e" "\<forall>e\<^sub>x. is_super_exp e e\<^sub>x \<longrightarrow> is_super_exp e\<^sub>l e\<^sub>x"
+
+    have "\<forall>e\<^sub>x. is_super_exp e\<^sub>l e\<^sub>x \<longrightarrow> is_super_exp (LET x = CASE x\<^sub>s LEFT x\<^sub>l |> e\<^sub>l RIGHT x\<^sub>r |> e\<^sub>r in e\<^sub>n) e\<^sub>x" by (simp add: is_super_exp.Let_Case_Left)
+    with `\<forall>e\<^sub>x. is_super_exp e e\<^sub>x \<longrightarrow> is_super_exp e\<^sub>l e\<^sub>x`
+    show "\<forall>e\<^sub>x. is_super_exp e e\<^sub>x \<longrightarrow> is_super_exp (LET x = CASE x\<^sub>s LEFT x\<^sub>l |> e\<^sub>l RIGHT x\<^sub>r |> e\<^sub>r in e\<^sub>n) e\<^sub>x" by blast
+  next
+    case (Let_Case_Right e\<^sub>r e x x\<^sub>s x\<^sub>l e\<^sub>l x\<^sub>r e\<^sub>n)
+    assume "is_super_exp e\<^sub>r e" "\<forall>e\<^sub>x. is_super_exp e e\<^sub>x \<longrightarrow> is_super_exp e\<^sub>r e\<^sub>x"
+
+    have "\<forall>e\<^sub>x. is_super_exp e\<^sub>r e\<^sub>x \<longrightarrow> is_super_exp (LET x = CASE x\<^sub>s LEFT x\<^sub>l |> e\<^sub>l RIGHT x\<^sub>r |> e\<^sub>r in e\<^sub>n) e\<^sub>x" by (simp add: is_super_exp.Let_Case_Right)
+    with `\<forall>e\<^sub>x. is_super_exp e e\<^sub>x \<longrightarrow> is_super_exp e\<^sub>r e\<^sub>x`
+    show "\<forall>e\<^sub>x. is_super_exp e e\<^sub>x \<longrightarrow> is_super_exp (LET x = CASE x\<^sub>s LEFT x\<^sub>l |> e\<^sub>l RIGHT x\<^sub>r |> e\<^sub>r in e\<^sub>n) e\<^sub>x" by blast
+  next
+    case (Let_Abs_Body e\<^sub>b e x f x\<^sub>p e\<^sub>n)
+    assume "is_super_exp e\<^sub>b e" "\<forall>e\<^sub>x. is_super_exp e e\<^sub>x \<longrightarrow> is_super_exp e\<^sub>b e\<^sub>x"
+
+    have "\<forall>e\<^sub>x. is_super_exp e\<^sub>b e\<^sub>x \<longrightarrow> is_super_exp (LET x = FN f x\<^sub>p . e\<^sub>b in e\<^sub>n) e\<^sub>x" by (simp add: is_super_exp.Let_Abs_Body)
+    with `\<forall>e\<^sub>x. is_super_exp e e\<^sub>x \<longrightarrow> is_super_exp e\<^sub>b e\<^sub>x`
+    show "\<forall>e\<^sub>x. is_super_exp e e\<^sub>x \<longrightarrow> is_super_exp (LET x = FN f x\<^sub>p . e\<^sub>b in e\<^sub>n) e\<^sub>x" by blast
+  qed 
+  with `is_super_exp e\<^sub>y e\<^sub>x`
+  show "is_super_exp e\<^sub>z e\<^sub>x" by blast
+qed
+
+lemma is_super_exp1: "
+  is_super_exp (LET x = b in e\<^sub>n) e\<^sub>n
+"
+by (simp add: Let Refl)
+
+
+fun val_to_bind :: "val \<Rightarrow> bind" where
+  "val_to_bind VUnit = \<lparr>\<rparr>" |
+  "val_to_bind (VChan _) = CHAN \<lparr>\<rparr>" |
+  "val_to_bind (VClosure p _) = Prim p"
+
+theorem static_traceable_implies_is_super_exp: "
+  \<lbrakk>
+    \<V> \<turnstile> e\<^sub>0 \<down> \<pi> \<mapsto> e;
+    (\<forall> x \<omega> . |\<omega>| \<in> \<V> x \<longrightarrow> (\<exists> x e\<^sub>n . is_super_exp e\<^sub>0 (LET x = val_to_bind \<omega> in e\<^sub>n )))
+  \<rbrakk> \<Longrightarrow>
+  is_super_exp e\<^sub>0 e 
+"
+proof -
+  assume "\<forall>x \<omega>. |\<omega>| \<in> \<V> x \<longrightarrow> (\<exists>x e\<^sub>n. is_super_exp e\<^sub>0 (LET x = val_to_bind \<omega> in e\<^sub>n ))"
+  assume "\<V> \<turnstile> e\<^sub>0 \<down> \<pi> \<mapsto> e" then
+  have "(\<forall> x \<omega> . |\<omega>| \<in> \<V> x \<longrightarrow> (\<exists> x e\<^sub>n . is_super_exp e\<^sub>0 (LET x = val_to_bind \<omega> in e\<^sub>n ))) \<longrightarrow> is_super_exp e\<^sub>0 e"
+  proof (induction rule: static_traceable.induct)
+    case (Start \<V> e\<^sub>0)
+    then show ?case by (simp add: Refl)
+  next
+    case (Result \<V> e\<^sub>0 \<pi> x \<pi>' x\<^sub>r b e\<^sub>n)
+    then show ?case sorry
+  next
+    case (Let_Unit \<V> e\<^sub>0 \<pi> x e\<^sub>n)
+    then show ?case sorry
+  next
+    case (Let_Chan \<V> e\<^sub>0 \<pi> x e\<^sub>n)
+    then show ?case sorry
+  next
+    case (Let_Prim \<V> e\<^sub>0 \<pi> x p e\<^sub>n)
+    then show ?case sorry
+  next
+    case (Let_Spawn_Child \<V> e\<^sub>0 \<pi> x e\<^sub>c e\<^sub>n)
+    then show ?case sorry
+  next
+    case (Let_Spawn \<V> e\<^sub>0 \<pi> x e\<^sub>c e\<^sub>n)
+    then show ?case sorry
+  next
+    case (Let_Sync \<V> e\<^sub>0 \<pi> x x\<^sub>v e\<^sub>n)
+    then show ?case sorry
+  next
+    case (Let_Fst \<V> e\<^sub>0 \<pi> x p e\<^sub>n)
+    then show ?case sorry
+  next
+    case (Let_Snd \<V> e\<^sub>0 \<pi> x p e\<^sub>n)
+    then show ?case sorry
+  next
+    case (Let_Case_Left \<V> e\<^sub>0 \<pi> x x\<^sub>s x\<^sub>l e\<^sub>l x\<^sub>r e\<^sub>r e\<^sub>n)
+    then show ?case sorry
+  next
+    case (Let_Case_Right \<V> e\<^sub>0 \<pi> x x\<^sub>s x\<^sub>l e\<^sub>l x\<^sub>r e\<^sub>r e\<^sub>n)
+    then show ?case sorry
+  next
+    case (Let_App \<V> e\<^sub>0 \<pi> x f x\<^sub>a e\<^sub>n f' x' e')
+    then show ?case sorry
+  qed
+    case (Start \<V> e\<^sub>0)
+    then show ?case
+    by (simp add: Refl)
+  next
+    case (Result \<V> e\<^sub>0 \<pi> x \<pi>' x\<^sub>r b e\<^sub>n)
+    then show ?case
+    using is_super_exp1 is_super_exp_trans by blast
+  next
+    case (Let_Unit \<V> e\<^sub>0 \<pi> x e\<^sub>n)
+    then show ?case
+    using is_super_exp1 is_super_exp_trans by blast
+  next
+    case (Let_Chan \<V> e\<^sub>0 \<pi> x e\<^sub>n)
+    then show ?case
+    using is_super_exp1 is_super_exp_trans by blast
+  next
+    case (Let_Prim \<V> e\<^sub>0 \<pi> x p e\<^sub>n)
+    then show ?case
+    using is_super_exp1 is_super_exp_trans by blast
+    next
+    case (Let_Spawn_Child \<V> e\<^sub>0 \<pi> x e\<^sub>c e\<^sub>n)
+    then show ?case
+    using Refl is_super_exp.Let_Spawn_Child is_super_exp_trans by blast
+  next
+    case (Let_Spawn \<V> e\<^sub>0 \<pi> x e\<^sub>c e\<^sub>n)
+    then show ?case
+    using is_super_exp1 is_super_exp_trans by blast
+  next
+      case (Let_Sync \<V> e\<^sub>0 \<pi> x x\<^sub>v e\<^sub>n)
+    then show ?case
+    using is_super_exp1 is_super_exp_trans by blast
+  next
+    case (Let_Fst \<V> e\<^sub>0 \<pi> x p e\<^sub>n)
+    then show ?case
+    using is_super_exp1 is_super_exp_trans by blast
+  next
+    case (Let_Snd \<V> e\<^sub>0 \<pi> x p e\<^sub>n)
+      then show ?case
+        using is_super_exp1 is_super_exp_trans by blast
+  next
+    case (Let_Case_Left \<V> e\<^sub>0 \<pi> x x\<^sub>s x\<^sub>l e\<^sub>l x\<^sub>r e\<^sub>r e\<^sub>n)
+    then show ?case
+      using Refl is_super_exp.Let_Case_Left is_super_exp_trans by blast
+  next
+    case (Let_Case_Right \<V> e\<^sub>0 \<pi> x x\<^sub>s x\<^sub>l e\<^sub>l x\<^sub>r e\<^sub>r e\<^sub>n)
+    then show ?case
+    using Refl is_super_exp.Let_Case_Right is_super_exp_trans by blast
+  next
+    case (Let_App \<V> e\<^sub>0 \<pi> x f x\<^sub>a e\<^sub>n)
+    then show ?case
+    by (metis (no_types, hide_lams) Let_Abs_Body Refl is_super_exp_trans val_to_bind.simps(3) value_to_abstract_value.simps(3))
+  qed
+  with `\<forall>x \<omega>. |\<omega>| \<in> \<V> x \<longrightarrow> (\<exists>x e\<^sub>n. LET x = val_to_bind \<omega> in e\<^sub>n is_super_exp e\<^sub>0)`
+  show "e is_super_exp e\<^sub>0"
+  by blast
+qed
 
 end
